Core/Vec.lean
@@ -115,10 +115,18 @@ theorem Vec.length_bound : (v : Vec A n) -> Vec.length v = n := by
   induction n <;> (simp at *)
 
 @[simp]
+theorem Vec.to_list_length : {v : Vec A n} -> (Vec.to_list v).length = n
+| .nil => by simp [Vec.to_list]
+| .cons hd tl =>
+  have lem := Vec.to_list_length (v := tl)
+  by grind [Vec.to_list]
+
+theorem Vec.eq_index_ext : {v1 v2 : Vec A n} -> (∀ (i : Fin n), v1[i] = v2[i]) -> v1 = v2 := sorry
+
+@[simp]
 def Vec.sum : Vec Nat n -> Nat
 | .nil => 0
 | .cons hd tl => hd + Vec.sum tl
-
 
 def Vec.rmap [i : RenMap S] (r : Ren) : Vec S n -> Vec S n
 | .nil => .nil
@@ -196,6 +204,16 @@ def Vec.seq : Vec (Option T) n -> Option (Vec T n)
 | .cons (some hd) tl => do
   let tl' <- Vec.seq tl
   return .cons hd tl'
+
+def Vec.range (n : Nat) : Vec Nat n := go n 0
+where
+  go : (n : Nat) -> Nat -> Vec Nat n
+  | 0, _ => .nil
+  | n + 1, acc => .cons acc (go n (acc + 1))
+
+@[simp]
+theorem Vec.range_zero : range 0 = .nil := sorry
+
 
 -- theorem Vec.seq_sound {vs : Vec n (Option Q)} {vs' : Vec n Q}:
 --   vs.seq = some vs' ->
